## Regra da cadeia:
## $\large  \color{green} \boxed {g'(x) = g'[h(x)] . h'(x)}$
>### A regra da cadeia é uma fórmula para a derivada da função composta de duas funções.

### Exemplos:

$$\Huge
{f(x) = ln(x^2+3x-10)}\\\,\\
{f'(x) = {1 \over x^2 + 3x - 10} \times {2x+3 =}}\\\,\\
{f'(x) = {2x+3 \over x^2+3x-10}}
$$(1)
---
$$\Huge 
{f(x) = 5e^{5x^3-x}}\\\,\\
{f'(x) = 5e^{5x^3-x}}
$$(2)
---
$$\Huge
{f(x) = \sin(\cos3x)}\\\,\\
{f'(x) = 3\times\cos(\cos3x)\times-\sin(3x)}
$$(3)
---
$$\Huge
{f(x) = \sec(3x+1)}\\\,\\
{f'(x) = 3\times\tg(3x+1)\times\sec(3x+1)}\\\,\\
{f'(x) = 3\times{\sin\over\cos^2}(3x+1)}
$$(4)